\documentclass{article}

% Packages
\usepackage[margin=1in]{geometry}
\usepackage{amsmath,amssymb}
\usepackage{titlesec}
\usepackage{titling}
\usepackage{mathtools}

% Custom unnumbered section format
\titleformat{\section}[block]
  {\normalfont\Large\bfseries}{}{0pt}{}  % Remove section number

% Left-aligned large title
\pretitle{\begin{flushleft}\LARGE\bfseries}
\posttitle{\end{flushleft}}
\preauthor{\begin{flushleft} \large}
\postauthor{\end{flushleft}}
\predate{\begin{flushleft} \large}
\postdate{\end{flushleft}}
\date{}

% Title info
\title{Appendix 1}
\begin{document}

\maketitle

\section{Transformation Law of the Metric} 

In this section, we deduce the transformation law for each 
individual component of the metric from a fully linear algebraic 
perspective. Recall that from the main paper, under transformation 
from coordinate $x$ to $x'$, the metric $M$ transforms according to 
\[
M' = J_{x' \mapsto x}^\top M J_{x' \mapsto x},
\tag{1}
\]
where $M'$ is the metric after transformation, and $J_{x' \mapsto x}$ 
represents the Jacobian matrix for the inverse transformation $x' \mapsto x$.
Taking $x$ as a function of $x'$: $x(x')$, we can write out the components 
of $J_{x' \mapsto x}$ as
\[
J_{x' \mapsto x} =
\begin{bmatrix}
\frac{\partial x^1}{\partial x^{\prime 1}} & \frac{\partial x^1}{\partial x^{\prime 2}} & \cdots & \frac{\partial x^1}{\partial x^{\prime n}} \\
\frac{\partial x^2}{\partial x^{\prime 1}} & \frac{\partial x^2}{\partial x^{\prime 2}} & \cdots & \frac{\partial x^2}{\partial x^{\prime n}} \\
\vdots & \vdots & \ddots & \vdots \\
\frac{\partial x^n}{\partial x^{\prime 1}} & \frac{\partial x^n}{\partial x^{\prime 2}} & \cdots & \frac{\partial x^n}{\partial x^{\prime n}} \\
\end{bmatrix}
\]
where $x^i$ and $x'^j$ denote the $i$-th coordinate function of $x$ and 
the $j$-th coordinate function of $x'$, respectively. Writing the component on the 
$\mu$-th row and $\nu$-th column as $g_{\mu\nu}$ for (1), we yield
\[
M' = 
\left[
\begin{array}{cccc}
\frac{\partial x^1}{\partial x^{\prime 1}} & \frac{\partial x^2}{\partial x^{\prime 1}} & \cdots & \frac{\partial x^n}{\partial x^{\prime 1}} \\
\frac{\partial x^1}{\partial x^{\prime 2}} & \frac{\partial x^2}{\partial x^{\prime 2}} & \cdots & \frac{\partial x^n}{\partial x^{\prime 2}} \\
\vdots & \vdots & \ddots & \vdots \\
\frac{\partial x^1}{\partial x^{\prime n}} & \frac{\partial x^2}{\partial x^{\prime n}} & \cdots & \frac{\partial x^n}{\partial x^{\prime n}} \\
\end{array}
\right]
\left[
\begin{array}{cccc}
g_{11} & g_{12} & \cdots & g_{1n} \vphantom{\frac{\partial x^1}{\partial x^{\prime n}}} \\
g_{21} & g_{22} & \cdots & g_{2n} \vphantom{\frac{\partial x^1}{\partial x^{\prime n}}} \\
\vdots & \vdots & \ddots & \vdots \\
g_{n1} & g_{n2} & \cdots & g_{nn} \vphantom{\frac{\partial x^1}{\partial x^{\prime n}}} \\
\end{array}
\right]
\left[
\begin{array}{cccc}
\frac{\partial x^1}{\partial x^{\prime 1}} & \frac{\partial x^1}{\partial x^{\prime 2}} & \cdots & \frac{\partial x^1}{\partial x^{\prime n}} \\
\frac{\partial x^2}{\partial x^{\prime 1}} & \frac{\partial x^2}{\partial x^{\prime 2}} & \cdots & \frac{\partial x^2}{\partial x^{\prime n}} \\
\vdots & \vdots & \ddots & \vdots \\
\frac{\partial x^n}{\partial x^{\prime 1}} & \frac{\partial x^n}{\partial x^{\prime 2}} & \cdots & \frac{\partial x^n}{\partial x^{\prime n}} \vphantom{\frac{\partial x^1}{\partial x^{\prime n}}} \\
\end{array}
\right]
\]
Now focus on the the matrix product $M J_{x' \mapsto x}$.
\begin{align*}
M J_{x' \mapsto x} &=
\left[
\begin{array}{cccc}
g_{11} & g_{12} & \cdots & g_{1n} \vphantom{\frac{\partial x^1}{\partial x^{\prime n}}} \\
g_{21} & g_{22} & \cdots & g_{2n} \vphantom{\frac{\partial x^1}{\partial x^{\prime n}}} \\
\vdots & \vdots & \ddots & \vdots \\
g_{n1} & g_{n2} & \cdots & g_{nn} \vphantom{\frac{\partial x^1}{\partial x^{\prime n}}} \\
\end{array}
\right]
\left[
\begin{array}{cccc}
\frac{\partial x^1}{\partial x^{\prime 1}} & \frac{\partial x^1}{\partial x^{\prime 2}} & \cdots & \frac{\partial x^1}{\partial x^{\prime n}} \\
\frac{\partial x^2}{\partial x^{\prime 1}} & \frac{\partial x^2}{\partial x^{\prime 2}} & \cdots & \frac{\partial x^2}{\partial x^{\prime n}} \\
\vdots & \vdots & \ddots & \vdots \\
\frac{\partial x^n}{\partial x^{\prime 1}} & \frac{\partial x^n}{\partial x^{\prime 2}} & \cdots & \frac{\partial x^n}{\partial x^{\prime n}} \vphantom{\frac{\partial x^1}{\partial x^{\prime n}}} \\
\end{array}
\right] \\\\
&=
\left[
\begin{array}{cccc}
\sum_{\lambda=1}^n g_{1\lambda} \frac{\partial x^\lambda}{\partial x^{\prime 1}} &
\sum_{\lambda=1}^n g_{1\lambda} \frac{\partial x^\lambda}{\partial x^{\prime 2}} &
\cdots &
\sum_{\lambda=1}^n g_{1\lambda} \frac{\partial x^\lambda}{\partial x^{\prime n}} \\
\sum_{\lambda=1}^n g_{2\lambda} \frac{\partial x^\lambda}{\partial x^{\prime 1}} &
\sum_{\lambda=1}^n g_{2\lambda} \frac{\partial x^\lambda}{\partial x^{\prime 2}} &
\cdots &
\sum_{\lambda=1}^n g_{2\lambda} \frac{\partial x^\lambda}{\partial x^{\prime n}} \\
\vdots & \vdots & \ddots & \vdots \\
\sum_{\lambda=1}^n g_{n\lambda} \frac{\partial x^\lambda}{\partial x^{\prime 1}} &
\sum_{\lambda=1}^n g_{n\lambda} \frac{\partial x^\lambda}{\partial x^{\prime 2}} &
\cdots &
\sum_{\lambda=1}^n g_{n\lambda} \frac{\partial x^\lambda}{\partial x^{\prime n}} \\
\end{array}
\right]
\end{align*}
Thus, denoting the entry at the $\mu$-th row, $\nu$-th column as $\tilde{g}_{\mu\nu}$,
we have
\[
\tilde{g}_{\mu\nu} = \sum_{\lambda=1}^n g_{\mu\lambda}
\frac{\partial x^\lambda}{\partial x^{\prime \nu}}
\tag{2}
\]\\

Similarly, for the entire $M'$,
\begin{align*}
M' &= 
\left[
\begin{array}{cccc}
\frac{\partial x^1}{\partial x^{\prime 1}} & \frac{\partial x^2}{\partial x^{\prime 1}} & \cdots & \frac{\partial x^n}{\partial x^{\prime 1}} \\
\frac{\partial x^1}{\partial x^{\prime 2}} & \frac{\partial x^2}{\partial x^{\prime 2}} & \cdots & \frac{\partial x^n}{\partial x^{\prime 2}} \\
\vdots & \vdots & \ddots & \vdots \\
\frac{\partial x^1}{\partial x^{\prime n}} & \frac{\partial x^2}{\partial x^{\prime n}} & \cdots & \frac{\partial x^n}{\partial x^{\prime n}} \\
\end{array}
\right]
M J_{x' \mapsto x} \\\\
&=
\left[
\begin{array}{cccc}
\frac{\partial x^1}{\partial x^{\prime 1}} & \frac{\partial x^2}{\partial x^{\prime 1}} & \cdots & \frac{\partial x^n}{\partial x^{\prime 1}} \\
\frac{\partial x^1}{\partial x^{\prime 2}} & \frac{\partial x^2}{\partial x^{\prime 2}} & \cdots & \frac{\partial x^n}{\partial x^{\prime 2}} \\
\vdots & \vdots & \ddots & \vdots \\
\frac{\partial x^1}{\partial x^{\prime n}} & \frac{\partial x^2}{\partial x^{\prime n}} & \cdots & \frac{\partial x^n}{\partial x^{\prime n}} \\
\end{array}
\right]
\left[
\begin{array}{cccc}
\tilde{g}_{11} & \tilde{g}_{12} & \cdots & \tilde{g}_{1n} \vphantom{\frac{\partial x^1}{\partial x^{\prime n}}} \\
\tilde{g}_{21} & \tilde{g}_{22} & \cdots & \tilde{g}_{2n} \vphantom{\frac{\partial x^1}{\partial x^{\prime n}}} \\
\vdots & \vdots & \ddots & \vdots \\
\tilde{g}_{n1} & \tilde{g}_{n2} & \cdots & \tilde{g}_{nn} \vphantom{\frac{\partial x^1}{\partial x^{\prime n}}} \\
\end{array}
\right] \\\\
&=
\left[
\begin{array}{cccc}
\sum_{\lambda=1}^n \tilde{g}_{\lambda 1} \frac{\partial x^\lambda}{\partial x^{\prime 1}} &
\sum_{\lambda=1}^n \tilde{g}_{\lambda 2} \frac{\partial x^\lambda}{\partial x^{\prime 1}} &
\cdots &
\sum_{\lambda=1}^n \tilde{g}_{\lambda n} \frac{\partial x^\lambda}{\partial x^{\prime 1}} \\
\sum_{\lambda=1}^n \tilde{g}_{\lambda 1} \frac{\partial x^\lambda}{\partial x^{\prime 2}} &
\sum_{\lambda=1}^n \tilde{g}_{\lambda 2} \frac{\partial x^\lambda}{\partial x^{\prime 2}} &
\cdots &
\sum_{\lambda=1}^n \tilde{g}_{\lambda n} \frac{\partial x^\lambda}{\partial x^{\prime 2}} \\
\vdots & \vdots & \ddots & \vdots \\
\sum_{\lambda=1}^n \tilde{g}_{\lambda 1} \frac{\partial x^\lambda}{\partial x^{\prime n}} &
\sum_{\lambda=1}^n \tilde{g}_{\lambda 2} \frac{\partial x^\lambda}{\partial x^{\prime n}} &
\cdots &
\sum_{\lambda=1}^n \tilde{g}_{\lambda n} \frac{\partial x^\lambda}{\partial x^{\prime n}}
\end{array}
\right],
\end{align*}
it would have entries
\[
g'_{\mu\nu} = \sum_{\lambda=1}^n \tilde{g}_{\lambda\nu}
\frac{\partial x^\lambda}{\partial x^{\prime \mu}}
\]
Now substitute in the expression for $\tilde{g}_{\lambda\nu}$, 
we obtain the components of $M'$:
\[
M' =
\left[
\begin{array}{cccc}
g'_{11} & g'_{12} & \cdots & g'_{1n} \vphantom{\frac{\partial x^1}{\partial x^{\prime n}}} \\
g'_{21} & g'_{22} & \cdots & g'_{2n} \vphantom{\frac{\partial x^1}{\partial x^{\prime n}}} \\
\vdots & \vdots & \ddots & \vdots \\
g'_{n1} & g'_{n2} & \cdots & g'_{nn} \vphantom{\frac{\partial x^1}{\partial x^{\prime n}}} \\
\end{array}
\right],
\]
where
\[
g'_{\mu\nu} = \sum_{\beta=1}^n 
\sum_{\alpha=1}^n g_{\alpha\beta} \frac{\partial x^\alpha}{\partial x'^\mu} 
\frac{\partial x^\beta}{\partial x'^\nu}
\]



\end{document}